\documentclass[a4paper, 12pt, reqno]{amsart}

\usepackage{amssymb}
\usepackage{amsfonts}
\numberwithin{equation}{section}
\usepackage[margin=1in]{geometry}
\usepackage[english]{babel}
\usepackage[colorlinks, pdftitle={Actuarial Mathematics Homework 3},
    pdfauthor={Moritz M. Konarski}]{hyperref}
\usepackage{enumitem}
\usepackage{graphicx}

\title{Actuarial Mathematics Homework 3}
\author{Moritz M. Konarski}
\date{\today}

\begin{document}

\maketitle

\subsection*{1--29}

\begin{enumerate}[label=(\alph*)]
    \item $i = 0.13 \rightarrow \delta = 0.122218$
    \item $d = 0.13 \rightarrow \delta = 0.139262$
    \item $i^{(4)} = 0.13 \rightarrow i = 0.136476 \rightarrow \delta
        = 0.127932$
    \item $d^{(5)} = 0.13 \rightarrow d = 0.123799 \rightarrow \delta
        = 0.132159$
\end{enumerate}

\subsection*{1--30}

Find derivatives
\begin{equation}\nonumber
    \begin{aligned}
        a(t) &= 1 + it - (1+i)^t \qquad (1+i)^t = e^{t \cdot \ln{(1+i)}}    \\
        &\qquad \delta = \ln{(1+i)}                                         \\
        a'(t) &= i - \left[ (1+i)^t \right]'_t                              \\
        a'(t) &= i - \left[ e^{t \cdot \ln{(1+i)}} \right]'                 \\
        a'(t) &= i -\ln{(1+i)} e^{t \cdot \ln{(1+i)}}                       \\
        a'(t) &= i -\delta e^{t \cdot \delta}                       \\
        a''(t) &=  \left[ -\ln{(1+i)} e^{t \cdot \ln{(1+i)}} \right]'       \\
        a''(t) &= -\left(\ln{(1+i)}\right)^2 \cdot e^{t \cdot \ln{(1+i)}}   \\
        a''(t) &= -\delta^2 \cdot e^{t \cdot \delta}
    \end{aligned}
\end{equation}

Find $a'(t) = 0$
\begin{equation}\nonumber
    \begin{aligned}
        a'(t_0) &= 0 \\
        0 &= i -\delta e^{t_0 \cdot \delta}                       \\
        i &= \delta e^{t_0 \cdot \delta}                          \\
        \ln{i} &= \ln{\delta} + \ln{e^{t_0 \cdot \delta}}         \\
        \ln{i} &= \ln{\delta} + t_0 \cdot \delta \cdot \ln{e}     \\
        t_0 &= \frac{\ln{i} - \ln{\delta}}{\delta} = 
            \frac{1}{\delta}[ \ln{i} - \ln{\delta}]
    \end{aligned}
\end{equation}

We found the same extremum as in the exercise. Now we need to show that it is
a maximum. For this we need $a''(t_0) < 0$
\begin{equation}\nonumber
    \begin{aligned}
        a''(t_0) &= -\delta^2 \cdot e^{t_0 \cdot \delta}        \\
        &= -\delta^2 \cdot e^{\frac{1}{\delta}[ \ln{i} - \ln{\delta}] 
            \cdot \delta}                                       \\
        &= -\delta^2 \cdot e^{\ln{i} - \ln{\delta}}             \\
        &= -\delta^2 \cdot (i / \delta)                         \\
        a''(t_0) &= -\delta \cdot i                  \\
        &\qquad \delta > 0, \quad i > 0       \\
        a''(t_0) &< 0    \qed
    \end{aligned}
\end{equation}


\subsection*{1--31}

\begin{enumerate}[label=(\alph*)]
    \item \begin{equation}\nonumber
            \begin{aligned}
                \delta = \ln{(1+i_0)}, &\qquad e^{\delta} = i_0 + 1      \\
                \delta_2 &= 2 \cdot \delta                              \\
                \delta_2 = \ln{(1+i_1)}, &\qquad e^{\delta_2} = i_1 + 1  \\
                i_1 = e^{\delta_2} - 1, &\qquad i_0 = e^{\delta} - 1    \\
                i_1 &> 2 \cdot i_0       \\
                e^{\delta_2} - 1 &> 2 \cdot \left( e^{\delta} - 1 \right)   \\
                \left(e^{\delta}\right)^2 &> 2 e^{\delta} - 1               \\
                \left(e^{\delta}\right)^2 -2 e^{\delta} + 1 &> 0        \\
                \left(e^{\delta} - 1\right)^2 &> 0                      \\
                e^{\delta} &> 1                       \\
                \delta &> 0                      \\
            \end{aligned}
        \end{equation}
    \item \begin{equation}\nonumber
            \begin{aligned}
                \delta = -\ln{(1-d_0)}, &\qquad e^{-\delta} = 1 - d_0      \\
                \delta_2 &= 2 \cdot \delta                              \\
                \delta_2 = -\ln{(1-d_1)}, &\qquad e^{-\delta_2} = 1-d_1  \\
                d_1 = -e^{-\delta_2} + 1, &\qquad d_0 = -e^{-\delta} + 1    \\
                d_1 &< 2 \cdot d_0       \\
                -e^{-\delta_2} + 1 &< 2 \cdot \left( -e^{-\delta} + 1 \right)\\
                \left(-e^{-\delta}\right)^2 + 1 &< -2e^{-\delta} + 2 \\
                0 &< \left(e^{-\delta}\right)^2 -2e^{-\delta} + 1 \\
                0 &< \left(e^{-\delta} - 1\right)^2\\
                e^{-\delta} &< 1                       \\
                -\delta &< 0                      \\
            \end{aligned}
        \end{equation}
\end{enumerate}

\subsection*{1--32}

\begin{equation}\nonumber
    \begin{aligned}
        \lim_{i \rightarrow 0} \frac{i-\delta}{\delta^2} &= 0.5  \\
        \lim_{i \rightarrow 0} \frac{i-\ln{(1+i)}}{(\ln{(1+i)})^2}&, \quad
            \text{we get} \quad \frac{0}{0}             \\
        \text{applying L'Hopital's Rule we get}& \\
        \lim_{i \rightarrow 0}
            \frac{1-\frac{1}{1+i}}{2\ln{(1+i)}\frac{1}{1+i}}&, \quad
            \text{we still get} \quad \frac{0}{0} \\
        \text{again applying L'Hopital's Rule we get}& \\
        \lim_{i \rightarrow 0}
            \frac{(1+i)^{-2}}{\left(2\ln{(1+i)}(1+i)^{-1}\right)'} &= \\
        \lim_{i \rightarrow 0}\frac{(1+i)^{-2}}{2((1+i)^{-2} - 
            \ln{(1+i)}(1+i)^{-2})} &= \\
        \lim_{i \rightarrow 0}\frac{(1+i)^{-2}}{2(1+i)^{-2}(1 - 
            \ln{(1+i)})} &= \\
        \lim_{i \rightarrow 0}\frac{1}{2(1 - \ln{(1+i)})} &= \frac{1}{2-0}
            = 0.5 
    \end{aligned}
\end{equation}

\subsection*{1--33}

\begin{equation}\nonumber
    \begin{aligned}
        \delta_t &= 0.04(1+t)^{-1}                  \\
        \delta_r &= 0.04(1+r)^{-1}                  \\
        a(t) &= e^{\int_0^t \delta_r dr}            \\
        \ln{(a(t))} &= \int_0^t{\delta_r}{dr}            \\
        &= \int_0^t{0.04(1+r)^{-1}}{dr}            \\
        &= 0.04 \int_0^t{(1+r)^{-1}}{dr}            \\
        &= 0.04 \left[\ln{(1+r)}\right]^t_0            \\
        &= 0.04 \left[\ln{(1+t)} - \ln{(1)}\right]            \\
        \ln{(a(t))} &= 0.04 \ln{(1+t)}                  \\
        a(t) &= (1+t)^{0.04}
    \end{aligned}
\end{equation}

\end{document}
