\documentclass[a4paper, 12pt, reqno]{amsart}

\usepackage{amsfonts}
\usepackage{amssymb}
\numberwithin{equation}{section}
\usepackage[margin=1in]{geometry}
\usepackage[english]{babel}
\usepackage[colorlinks, pdftitle={Homework 08.09.2020 Fixed}, 
    pdfauthor={Moritz M. Konarski}]{hyperref}
\renewcommand{\baselinestretch}{1.5}

\title{Num--Meth MAT--410: HW 08.09.20 Fixed 2}
\author{Moritz M. Konarski}
\date{\today}

\begin{document}

\maketitle

\section{Problem}

Solve 

\begin{equation}\nonumber
    \epsilon u'' + a u' = f(x)
\end{equation}

for the parameters

\begin{equation}\nonumber
    \begin{aligned}
        a &= 1 \qquad \text{and} \\
        f(x) &= x^3.
    \end{aligned}
\end{equation}

This gives

\begin{equation}\label{eq:01}
    u'' + \frac{u'}{\epsilon} = \frac{x^3}{\epsilon}.
\end{equation}

Consider the boundary conditions

\begin{equation}\nonumber
    \begin{cases}
        \phi_0 &= \zeta_0 u(0) - \eta_0 \epsilon u'(0) \qquad \text{and} \\
        \phi_1 &= \zeta_1 u(1) + \eta_1 \epsilon u'(1)
    \end{cases}
\end{equation}

for the cases 

\begin{equation}\nonumber
    \begin{cases}
        \zeta_0 = \zeta_1 = 1 \quad&; \quad \eta_0 = \eta_1 = 0 \qquad
        \text{and} \\
        \zeta_0 = \eta_0 = 1 \quad&; \quad \zeta_1 = 1, \text{ }\eta_1 = 0.
    \end{cases}
\end{equation}

This yields two cases. Case 1 is

\begin{equation}\label{eq:bvp1}
    \begin{cases}
        \phi_0 &= u(0) \\
        \phi_1 &= u(1)
    \end{cases}
\end{equation}

and case 2 is

\begin{equation}\label{eq:bvp2}
    \begin{cases}
        \phi_0 &= u(0) - \epsilon u'(0) \\
        \phi_1 &= u(1)
    \end{cases}
\end{equation}

\section{General Solution to Equation (\ref{eq:01})}

\subsection{Homogeneous Solution}

Solve (\ref{eq:01}) as a homogeneous equation in the form

\begin{equation}\label{eq:02}
    u_H = c_1 e^{\lambda_1} + c_2 e^{\lambda_2}.
\end{equation}

Find the $\lambda$s

\begin{equation}\nonumber
    \begin{aligned}
        \epsilon u'' + u' &= 0          \\
        u'' + \frac{1}{\epsilon} u' &= 0 \\
        \lambda^2 + \frac{1}{\epsilon} \lambda &= 0 \\
        \lambda_1 = 0 \quad & \quad \lambda_2 = - \frac{1}{\epsilon}.
    \end{aligned}
\end{equation}

Now substitute the $\lambda$s into (\ref{eq:02}) and find the homogeneous
solution

\begin{equation}\label{eq:hom}
    \begin{aligned}
        u_H &= c_1 + c_2 e^{-1/\epsilon \cdot x} \\
        u_1 = 1 &\qquad u_2 = e^{-1/\epsilon \cdot x}.
    \end{aligned}
\end{equation}

\subsection{Particular Solution}

Using the variation of parameters method we can find the particular solution
with the help of (\ref{eq:hom})

\begin{equation}\nonumber
    \begin{aligned}
        u_P &= -u_1 \int{\frac{u_2 f(x)}{W(u_1,u_2)}}{dx} + 
            u_2 \int{\frac{u_1 f(x)}{W(u_1,u_2)}}{dx}           \\
        &W(u_1,u_2) = u_1 u_2' - u_2 u_1' = 
            -\frac{1}{\epsilon}e^{-1/\epsilon \cdot x}.
    \end{aligned}
\end{equation}

Plugging in $W$ and cancelling, we get 

\begin{equation}\nonumber
    \begin{aligned}
        u_P &= - \int{\frac{e^{-1/\epsilon\cdot x}\frac{1}{\epsilon}x^3}
            {-\frac{1}{\epsilon}e^{-1/\epsilon \cdot x}}}{dx} 
            + e^{-1/\epsilon \cdot x} \int{\frac{\frac{1}{\epsilon} x^3}
                {-\frac{1}{\epsilon}e^{-1/\epsilon \cdot x}}}{dx} \\
        u_P &= \int{x^3}{dx} - e^{-1/\epsilon \cdot x} 
            \int{x^3 \cdot e^{1/\epsilon \cdot x}}{dx}.
    \end{aligned}
\end{equation}

From here 3 rounds of integration by parts results in 

\begin{equation}\nonumber
    u_P = \frac{1}{4}x^4 - e^{-1/\epsilon \cdot x} 
        \left[ \epsilon x^3 e^{1/\epsilon \cdot x} -3\epsilon
        \left[ \epsilon x^2 e^{1/\epsilon \cdot x} -2\epsilon
        \left[ \epsilon x   e^{1/\epsilon \cdot x} -\epsilon
        \left(  \epsilon    e^{1/\epsilon \cdot x} \right) 
        \right] \right] \right]
\end{equation}

which can be reduced to 

\begin{equation}\label{eq:part}
    u_P = \frac{1}{4}x^4 - \epsilon x^3 + 3\epsilon^2 x^2 
        - 6 \epsilon^3 x + 6 \epsilon^4.
\end{equation}

Now we can find the complete solution by adding the homogeneous solution
(\ref{eq:hom}) and the particular solution (\ref{eq:part}) together

\begin{equation}\label{eq:comp}
    \begin{aligned}
        u &= u_H + u_P \\
        u &= c_1 + c_2 \cdot e^{-1/\epsilon \cdot x} + \frac{1}{4}x^4 
            - \epsilon x^3 + 3\epsilon^2 x^2 - 6 \epsilon^3 x + 6 \epsilon^4 \\
        u' &= -\frac{1}{\epsilon} c_2 e^{-1/\epsilon \cdot x} + x^3 
            - 3 \epsilon x^2 + 6\epsilon^2 x - 6 \epsilon^3
    \end{aligned}
\end{equation}

\section{Solution to BVP 1}

Combining (\ref{eq:bvp1}) with (\ref{eq:comp}) yields

\begin{equation}\nonumber
    \begin{aligned}
        \phi_0 &= u(0) = c_1 + c_2 + 6 \epsilon^4       \\
        \phi_1 &= u(1) = c_1 + c_2 e^{-1/\epsilon} + \frac{1}{4} - \epsilon 
            + 3 \epsilon^2 - 6 \epsilon^3 + 6 \epsilon^4.
    \end{aligned}
\end{equation}

Rearranging the equations we get

\begin{equation}\nonumber
    \begin{aligned}
        c_1 &= \phi_0 - 6 \epsilon^4 - \frac{\phi_0 - \phi_1 + 1/4 - \epsilon 
            + 3 \epsilon^2 - 6 \epsilon^3}{1 - e^{-1/\epsilon}}     \\
        c_2 &= \frac{\phi_0 - \phi_1 + 1/4 - \epsilon + 3 \epsilon^2 
            - 6 \epsilon^3}{1 - e^{-1/\epsilon}}.
    \end{aligned}
\end{equation}

Plugging $c_1$ and $c_2$ into (\ref{eq:comp}) yields

\begin{equation}\nonumber
    \begin{aligned}
    u &= \phi_0 - 6 \epsilon^4 - \frac{\phi_0 - \phi_1 + 1/4 - \epsilon 
            + 3 \epsilon^2 - 6 \epsilon^3}{1 - e^{-1/\epsilon}}     \\
        &+ \frac{\phi_0 - \phi_1 + 1/4 - \epsilon + 3 \epsilon^2 
            - 6 \epsilon^3}{1 - e^{-1/\epsilon}} \cdot e^{-1/\epsilon \cdot x}\\
        &+ \frac{1}{4}x^4 - \epsilon x^3 + 3\epsilon^2 x^2 
        - 6 \epsilon^3 x + 6 \epsilon^4                     \\
        u &= (e^{-1/\epsilon\cdot x} - 1) 
            \frac{\phi_0 - \phi_1 + 1/4 - \epsilon+3 \epsilon^2
            - 6 \epsilon^3} {1 - e^{-1/\epsilon}}\\
         &+ \frac{1}{4}x^4-\epsilon x^3+3\epsilon^2 x^2-6\epsilon^3 x+\phi_0
    \end{aligned}
\end{equation}

\section{Solution to BVP 2}

Combining (\ref{eq:bvp2}) with (\ref{eq:comp}) yields

\begin{equation}\nonumber
    \begin{aligned}
        \phi_0 &= u(0) -\epsilon u'(0) = c_1 + 2 c_2 + 12 \epsilon^4  \\
        \phi_1 &= u(1) = c_1 + c_2 e^{-1/\epsilon} + \frac{1}{4} - \epsilon 
            + 3 \epsilon^2 - 6 \epsilon^3 + 6 \epsilon^4.
    \end{aligned}
\end{equation}

Rearranging the equations we get

\begin{equation}\nonumber
    \begin{aligned}
        c_1 &= \phi_0  - 12 \epsilon^4 - 2 \left( \frac{\phi_0-\phi_1+1/4
            -\epsilon+3\epsilon^2-6\epsilon^3-6\epsilon^4}{2 - e^{-1/\epsilon}}
            \right)       \\
        c_2 &= \frac{\phi_0-\phi_1+1/4-\epsilon+3\epsilon^2-6\epsilon^3
            -6\epsilon^4}{2 - e^{-1/\epsilon}}.
    \end{aligned}
\end{equation}

Plugging $c_1$ and $c_2$ into (\ref{eq:comp}) yields

\begin{equation}\nonumber
    \begin{aligned}
    u &= \phi_0  - 12 \epsilon^4 - 2 \left( \frac{\phi_0-\phi_1+1/4
            -\epsilon+3\epsilon^2-6\epsilon^3-6\epsilon^4}{2 - e^{-1/\epsilon}}
            \right)       \\
        &+ \frac{\phi_0-\phi_1+1/4-\epsilon+3\epsilon^2-6\epsilon^3
            -6\epsilon^4}{2 - e^{-1/\epsilon}} \cdot e^{-1/\epsilon \cdot x}\\
        &+ \frac{1}{4}x^4 - \epsilon x^3 + 3\epsilon^2 x^2 
            - 6 \epsilon^3 x + 6 \epsilon^4             \\
        u &= \phi_0  + (e^{-1/\epsilon \cdot x} - 2) 
            \frac{\phi_0-\phi_1+1/4 -\epsilon+3\epsilon^2-6\epsilon^3-
            6\epsilon^4}{2 - e^{-1/\epsilon}}    \\
        &+ \frac{1}{4}x^4 - \epsilon x^3 + 3\epsilon^2 x^2 
            - 6 \epsilon^3 x - 6 \epsilon^4
    \end{aligned}
\end{equation}

\end{document}
